WIP

ems/Skeleton.v
@@ -1,7 +1,6 @@
 Require Import Coqlib.
 Require Export ZArith.
 Require Import String.
-Require Import PCM.
 Require Export AList.
 
 Set Implicit Arguments.
@@ -9,7 +8,9 @@ Set Implicit Arguments.
 Local Open Scope nat_scope.
 
 Notation gname := string (only parsing). (*** convention: not capitalized ***)
-Notation mname := string (only parsing). (*** convention: capitalized ***)
+Variant mname := | mn_some: string -> mname | mn_core. (*** convention: capitalized ***)
+Coercion mn_some: string >-> mname.
+Global Program Instance mname_Dec: Dec mname. Next Obligation. decide equality. eapply string_Dec. Defined.
 
 
 Fixpoint _find_idx {A} (f: A -> bool) (l: list A) (acc: nat): option (nat * A) :=
