ems/ModSem.v
@@ -32,13 +32,12 @@ Section MODSEML.
 
   Record t: Type := mk {
     (* initial_ld: mname -> GRA; *)
-    fnsems: alist gname ((option mname * Any.t) -> itree Es Any.t);
+    fnsems: alist gname ((mname * Any.t) -> itree Es Any.t);
     initial_mrs: alist mname Any.t;
   }
   .
 
   Record wf (ms: t): Prop := mk_wf {
-    wf_fnsems: NoDup (List.map fst ms.(fnsems));
     wf_initial_mrs: NoDup (List.map fst ms.(initial_mrs));
   }
   .
@@ -62,7 +61,9 @@ Section MODSEML.
 
   Definition prog: callE ~> itree Es :=
     fun _ '(Call mn fn args) =>
-      sem <- (alist_find fn ms.(fnsems))?;;
+      n <- trigger (Take _);;
+      assume(exists sem, nth_error ms.(fnsems) n = Some (fn, sem));;;
+      '(_, sem) <- (nth_error ms.(fnsems) n)?;;
       rv <- (sem (mn, args));;
       Ret rv
   .
@@ -81,7 +82,7 @@ Section MODSEML.
     | None => Ret tt
     | Some P' => assume (<<WF: P'>>)
     end;;;
-    snd <$> interp_Es prog (prog (Call None "main" initial_arg)) (initial_p_state).
+    snd <$> interp_Es prog (prog (Call mn_core "main" initial_arg)) (initial_p_state).
 
 
 
@@ -288,121 +289,6 @@ Section MODSEML.
   (* Next Obligation. inv STEP; ss. Qed. *)
 
   End INTERP.
-
-  (*** TODO: probably we can make ModSemL.t as an RA too. (together with Sk.t) ***)
-  (*** However, I am not sure what would be the gain; and there might be universe problem. ***)
-
-  Context {CONF: EMSConfig}.
-
-  Let add_comm_aux
-      ms0 ms1 stl0 str0
-      P
-      (SIM: stl0 = str0)
-    :
-      <<COMM: Beh.of_state (compile (add ms0 ms1) P) stl0
-              <1=
-              Beh.of_state (compile (add ms1 ms0) P) str0>>
-  .
-  Proof.
-    subst. revert str0. pcofix CIH. i. pfold.
-    punfold PR. induction PR using Beh.of_state_ind; ss.
-    - econs 1; et.
-    - econs 2; et.
-      clear CIH. clear_tac. revert st0 H.
-      pcofix CIH. i. punfold H0. pfold.
-      inv H0.
-      + econs 1; eauto. ii. ss. exploit STEP; et. i; des. right. eapply CIH; et. pclearbot. ss.
-      + econs 2; eauto. des. esplits; eauto. right. eapply CIH; et. pclearbot. ss.
-    - econs 4; et. pclearbot. right. eapply CIH; et.
-    - econs 5; et. rr in STEP. des. rr. esplits; et.
-    - econs 6; et. ii. exploit STEP; et. i; des. clarify.
-  Qed.
-
-  Lemma wf_comm
-        ms0 ms1
-    :
-      <<EQ: wf (add ms0 ms1) = wf (add ms1 ms0)>>
-  .
-  Proof.
-    assert (forall ms0 ms1, wf (add ms0 ms1) -> wf (add ms1 ms0)).
-    { i. inv H. econs; ss.
-      { rewrite List.map_app in *.
-        eapply nodup_comm; et. }
-      { rewrite List.map_app in *.
-        eapply nodup_comm; et. }
-    }
-    r. eapply prop_ext. split; i; auto.
-  Qed.
-
-  Theorem add_comm
-          ms0 ms1 (P0 P1: Prop) (IMPL: P1 -> P0)
-          (WF: wf (add ms1 ms0))
-    :
-      <<COMM: Beh.of_program (compile (add ms0 ms1) (Some P0)) <1= Beh.of_program (compile (add ms1 ms0) (Some P1))>>
-  .
-  Proof.
-    destruct (classic (P1)); cycle 1.
-    { ii. eapply initial_itr_not_wf; et. }
-    replace P0 with P1.
-    2: { eapply prop_ext. split; auto. }
-    ii. ss. r in PR. r. eapply add_comm_aux; et.
-    rp; et. clear PR. ss. cbn. unfold initial_itr. f_equal.
-    { extensionality u. destruct u. f_equal.
-      replace (@interp_Es Any.t (prog (add ms1 ms0))) with (@interp_Es Any.t (prog (add ms0 ms1))).
-      { f_equal.
-        { ss. f_equal. f_equal. eapply alist_permutation_find.
-          { inv WF. et. }
-          { eapply Permutation_app_comm. }
-        }
-        { unfold initial_p_state. extensionality mn. ss.
-          erewrite alist_permutation_find; et.
-          { inv WF. ss. }
-          { eapply Permutation_app_comm. }
-        }
-      }
-      f_equal. unfold prog. extensionality T. extensionality e. destruct e.
-      f_equal. f_equal. symmetry. eapply alist_permutation_find; et.
-      { inv WF. ss. }
-      { eapply Permutation_app_comm. }
-    }
-  Qed.
-
-  Lemma add_assoc' ms0 ms1 ms2:
-    add ms0 (add ms1 ms2) = add (add ms0 ms1) ms2.
-  Proof.
-    induction ms2; ss. unfold add. f_equal; ss.
-    { eapply app_assoc. }
-    { eapply app_assoc. }
-  Qed.
-
-  Lemma add_assoc_eq ms0 ms1 ms2
-    :
-      add ms0 (add ms1 ms2) = add (add ms0 ms1) ms2.
-  Proof.
-    unfold add. ss. f_equal.
-    { apply List.app_assoc. }
-    { apply List.app_assoc. }
-  Qed.
-
-  Theorem add_assoc
-          ms0 ms1 ms2 P
-    :
-      <<COMM: Beh.of_program (compile (add ms0 (add ms1 ms2)) P) <1=
-              Beh.of_program (compile (add (add ms0 ms1) ms2) P)>>
-  .
-  Proof.
-    rewrite add_assoc_eq. ss.
-  Qed.
-
-  Theorem add_assoc_rev
-          ms0 ms1 ms2 P
-    :
-      <<COMM: Beh.of_program (compile (add ms0 (add ms1 ms2)) P) <1=
-              Beh.of_program (compile (add (add ms0 ms1) ms2) P)>>
-  .
-  Proof.
-    rewrite add_assoc_eq. ss.
-  Qed.
 End MODSEML.
 End ModSemL.
 
@@ -445,7 +331,7 @@ Section EVENTS.
 
   Definition handle_callE (mn: mname) `{EventsL.callE -< E}: callE ~> itree E :=
     fun _ '(Call fn args) =>
-      r <- trigger (EventsL.Call (Some mn) fn args);;
+      r <- trigger (EventsL.Call mn fn args);;
       Ret r
   .
 
@@ -496,7 +382,7 @@ Section EVENTS.
         fn args
     :
       transl_all mn (trigger (Call fn args)) =
-      r <- (trigger (EventsL.Call (Some mn) fn args));;
+      r <- (trigger (EventsL.Call mn fn args));;
       tau;; Ret r
   .
   Proof. unfold transl_all. rewrite unfold_interp. ss. grind. Qed.
@@ -553,9 +439,9 @@ Section EVENTSCOMMON.
   Definition ccallN {X Y} (fn: gname) (varg: X): itree E Y := vret <- trigger (Call fn varg↑);; vret <- vret↓ǃ;; Ret vret.
   Definition ccallU {X Y} (fn: gname) (varg: X): itree E Y := vret <- trigger (Call fn varg↑);; vret <- vret↓?;; Ret vret.
 
-  Definition cfunN {X Y} (body: X -> itree E Y): (option mname * Any.t) -> itree E Any.t :=
+  Definition cfunN {X Y} (body: X -> itree E Y): (mname * Any.t) -> itree E Any.t :=
     fun '(_, varg) => varg <- varg↓ǃ;; vret <- body varg;; Ret vret↑.
-  Definition cfunU {X Y} (body: X -> itree E Y): (option mname * Any.t) -> itree E Any.t :=
+  Definition cfunU {X Y} (body: X -> itree E Y): (mname * Any.t) -> itree E Any.t :=
     fun '(_, varg) => varg <- varg↓?;; vret <- body varg;; Ret vret↑.
 
 End EVENTSCOMMON.
@@ -566,7 +452,7 @@ Module ModSem.
 (* Import Events. *)
 Section MODSEM.
   Record t: Type := mk {
-    fnsems: list (gname * ((option mname * Any.t) -> itree Es Any.t));
+    fnsems: list (gname * ((mname * Any.t) -> itree Es Any.t));
     mn: mname;
     initial_st: Any.t;
   }
@@ -574,7 +460,9 @@ Section MODSEM.
 
   Definition prog (ms: t): callE ~> itree Es :=
     fun _ '(Call fn args) =>
-      sem <- (alist_find fn ms.(fnsems))?;;
+      n <- trigger (Take _);;
+      assume(exists sem, nth_error ms.(fnsems) n = Some (fn, sem));;;
+      '(_, sem) <- (nth_error ms.(fnsems) n)?;;
       '(mn, args) <- (Any.split args)ǃ;; mn <- mn↓ǃ;;
       (sem (mn, args))
   .
@@ -639,55 +527,6 @@ Section MODL.
   |}
   .
 
-  Theorem add_comm
-          md0 md1
-    :
-      <<COMM: Beh.of_program (compile (add md0 md1)) <1= Beh.of_program (compile (add md1 md0))>>
-  .
-  Proof.
-    ii. unfold compile in *.
-    destruct (classic (ModSemL.wf (enclose (add md1 md0)) /\ Sk.wf (sk (add md1 md0)))).
-    2: { eapply ModSemL.initial_itr_not_wf. ss. }
-    ss. des. assert (SK: Sk.wf (Sk.add (sk md0) (sk md1))).
-    { apply Sk.wf_comm. auto. }
-    rewrite Sk.add_comm; et.
-    eapply ModSemL.add_comm; [| |et].
-    { i. split; auto. unfold enclose. ss. rewrite Sk.add_comm; et.
-      inv H2. inv H3. econs; ss.
-      { rewrite List.map_app in *. eapply nodup_comm; et. }
-      { rewrite List.map_app in *. eapply nodup_comm; et. }
-    }
-    { rewrite Sk.add_comm; et. }
-  Qed.
-
-  Lemma add_assoc' ms0 ms1 ms2:
-    add ms0 (add ms1 ms2) = add (add ms0 ms1) ms2.
-  Proof.
-    unfold add. f_equal.
-    { extensionality skenv_link. ss. apply ModSemL.add_assoc'. }
-    { ss. rewrite Sk.add_assoc. auto. }
-  Qed.
-
-  Theorem add_assoc
-          md0 md1 md2
-    :
-      <<COMM: Beh.of_program (compile (add md0 (add md1 md2))) =
-              Beh.of_program (compile (add (add md0 md1) md2))>>
-  .
-  Proof.
-    rewrite add_assoc'. ss.
-  Qed.
-
-  Theorem add_assoc_rev
-          md0 md1 md2
-    :
-      <<COMM: Beh.of_program (compile (add (add md0 md1) md2)) =
-              Beh.of_program (compile (add md0 (add md1 md2)))>>
-  .
-  Proof.
-    rewrite add_assoc'. ss.
-  Qed.
-
   Definition empty: t := {|
     get_modsem := fun _ => ModSemL.mk [] [];
     sk := Sk.unit;
@@ -751,29 +590,6 @@ Section MOD.
        (add_list (x :: xs)) = (ModL.add x (add_list xs))
    .
    Proof. ss. Qed.
-
-   Lemma add_list_snoc
-         x xs
-     :
-       (add_list (snoc xs x)) = (ModL.add (add_list xs) x)
-   .
-   Proof.
-     ginduction xs; ii; ss.
-     { cbn. rewrite ModL.add_empty_l. rewrite ModL.add_empty_r. refl. }
-     { cbn. rewrite <- ModL.add_assoc'. f_equal. rewrite <- IHxs. refl. }
-   Qed.
-
-   Lemma add_list_app
-         xs ys
-     :
-       add_list (xs ++ ys) = ModL.add (add_list xs) (add_list ys)
-   .
-   Proof.
-     (* unfold add_list. rewrite map_app. rewrite fold_right_app. *)
-     ginduction xs; ii; ss.
-     - cbn. rewrite ModL.add_empty_l. refl.
-     - rewrite ! add_list_cons. rewrite <- ModL.add_assoc'. f_equal. eapply IHxs; ss.
-   Qed.
 
    Lemma add_list_sk (mdl: list t)
      :
@@ -912,272 +728,6 @@ pqrname :=
   (* . *)
 End Equisatisfiability.
 
-
-Section REFINE.
-  Context `{Sk.ld}.
-
-   Definition refines {CONF: EMSConfig} (md_tgt md_src: ModL.t): Prop :=
-     (* forall (ctx: list Mod.t), Beh.of_program (ModL.compile (add_list (md_tgt :: ctx))) <1= *)
-     (*                           Beh.of_program (ModL.compile (add_list (md_src :: ctx))) *)
-     forall (ctx: list Mod.t), Beh.of_program (ModL.compile (ModL.add (Mod.add_list ctx) md_tgt)) <1=
-                               Beh.of_program (ModL.compile (ModL.add (Mod.add_list ctx) md_src))
-   .
-
-   Definition refines_strong (md_tgt md_src: ModL.t): Prop :=
-     forall {CONF: EMSConfig}, refines md_tgt md_src.
-
-   Section CONF.
-   Context {CONF: EMSConfig}.
-
-   Definition refines2 (md_tgt md_src: list Mod.t): Prop :=
-     forall (ctx: list Mod.t), Beh.of_program (ModL.compile (ModL.add (Mod.add_list ctx) (Mod.add_list md_tgt))) <1=
-                               Beh.of_program (ModL.compile (ModL.add (Mod.add_list ctx) (Mod.add_list md_src)))
-   .
-
-   Global Program Instance refines2_PreOrder: PreOrder refines2.
-   Next Obligation.
-     ii. ss.
-   Qed.
-   Next Obligation.
-     ii. eapply H0 in PR. eapply H1 in PR. eapply PR.
-   Qed.
-
-   (*** vertical composition ***)
-   Global Program Instance refines_PreOrder: PreOrder refines.
-   Next Obligation. ii. ss. Qed.
-   Next Obligation. ii. eapply H1. eapply H0. ss. Qed.
-
-   Global Program Instance refines_strong_PreOrder: PreOrder refines_strong.
-   Next Obligation. ii. ss. Qed.
-   Next Obligation. ii. eapply H1. eapply H0. ss. Qed.
-
-
-
-   (*** horizontal composition ***)
-   Theorem refines_add
-         (md0_src md0_tgt md1_src md1_tgt: Mod.t)
-         (SIM0: refines md0_tgt md0_src)
-         (SIM1: refines md1_tgt md1_src)
-     :
-       <<SIM: refines (ModL.add md0_tgt md1_tgt) (ModL.add md0_src md1_src)>>
-   .
-   Proof.
-     ii. r in SIM0. r in SIM1.
-     (***
-ctx (a0 b0)
-(ctx a0) b0
-(ctx a0) b1
-      ***)
-     rewrite ModL.add_assoc in PR.
-     specialize (SIM1 (snoc ctx md0_tgt)). spc SIM1. rewrite Mod.add_list_snoc in SIM1. eapply SIM1 in PR.
-     (***
-ctx (a0 b1)
-(a0 b1) ctx
-a0 (b1 ctx)
-(b1 ctx) a0
-      ***)
-     rewrite <- ModL.add_assoc' in PR.
-     eapply ModL.add_comm in PR.
-     rewrite <- ModL.add_assoc' in PR.
-     eapply ModL.add_comm in PR.
-     (***
-(b1 ctx) a1
-a1 (b1 ctx)
-(a1 b1) ctx
-ctx (a1 b1)
-      ***)
-     specialize (SIM0 (cons md1_src ctx)). spc SIM0. rewrite Mod.add_list_cons in SIM0. eapply SIM0 in PR.
-     eapply ModL.add_comm in PR.
-     rewrite ModL.add_assoc' in PR.
-     eapply ModL.add_comm in PR.
-     ss.
-   Qed.
-
-   Theorem refines_proper_r
-         (mds0_src mds0_tgt: list Mod.t) (ctx: list Mod.t)
-         (SIM0: refines (Mod.add_list mds0_tgt) (Mod.add_list mds0_src))
-     :
-       <<SIM: refines (ModL.add (Mod.add_list mds0_tgt) (Mod.add_list ctx)) (ModL.add (Mod.add_list mds0_src) (Mod.add_list ctx))>>
-   .
-   Proof.
-     ii. r in SIM0. rename ctx into xs. rename ctx0 into ys.
-     (***
-ys + (tgt + xs)
-(tgt + xs) + ys
-tgt + (xs + ys)
-(xs + ys) + tgt
-      ***)
-     eapply ModL.add_comm in PR.
-     rewrite <- ModL.add_assoc' in PR.
-     eapply ModL.add_comm in PR.
-     (***
-(xs + ys) + src
-src + (xs + ys)
-(src + xs) + ys
-ys + (src + xs)
-      ***)
-     specialize (SIM0 (xs ++ ys)). spc SIM0. rewrite Mod.add_list_app in SIM0. eapply SIM0 in PR.
-     eapply ModL.add_comm in PR.
-     rewrite ModL.add_assoc' in PR.
-     eapply ModL.add_comm in PR.
-     ss.
-   Qed.
-
-   Theorem refines_proper_l
-         (mds0_src mds0_tgt: list Mod.t) (ctx: list Mod.t)
-         (SIM0: refines (Mod.add_list mds0_tgt) (Mod.add_list mds0_src))
-     :
-       <<SIM: refines (ModL.add (Mod.add_list ctx) (Mod.add_list mds0_tgt)) (ModL.add (Mod.add_list ctx) (Mod.add_list mds0_src))>>
-   .
-   Proof.
-     ii. r in SIM0. rename ctx into xs. rename ctx0 into ys.
-     (***
-ys + (xs + tgt)
-(ys + xs) + tgt
-(ys + xs) + src
-ys + (xs + src)
-      ***)
-     rewrite ModL.add_assoc' in PR.
-     specialize (SIM0 (ys ++ xs)). spc SIM0. rewrite Mod.add_list_app in SIM0. eapply SIM0 in PR.
-     rewrite <- ModL.add_assoc' in PR.
-     ss.
-   Qed.
-
-   Definition refines_closed (md_tgt md_src: ModL.t): Prop :=
-     Beh.of_program (ModL.compile md_tgt) <1= Beh.of_program (ModL.compile md_src)
-   .
-
-   Global Program Instance refines_closed_PreOrder: PreOrder refines_closed.
-   Next Obligation. ii; ss. Qed.
-   Next Obligation. ii; ss. eapply H1. eapply H0. eauto. Qed.
-
-   Lemma refines_close: refines <2= refines_closed.
-   Proof. ii. specialize (PR nil). ss. unfold Mod.add_list in *. ss. rewrite ! ModL.add_empty_l in PR. eauto. Qed.
-
-   (*** horizontal composition ***)
-   Theorem refines2_add
-         (s0 s1 t0 t1: list Mod.t)
-         (SIM0: refines2 t0 s0)
-         (SIM1: refines2 t1 s1)
-     :
-       <<SIM: refines2 (t0 ++ t1) (s0 ++ s1)>>
-   .
-   Proof.
-     ii. r in SIM0. r in SIM1.
-     (***
-ctx (a0 b0)
-(ctx a0) b0
-(ctx a0) b1
-      ***)
-     rewrite Mod.add_list_app in PR.
-     rewrite ModL.add_assoc in PR.
-     specialize (SIM1 (ctx ++ t0)). spc SIM1. rewrite Mod.add_list_app in SIM1. eapply SIM1 in PR.
-     (***
-ctx (a0 b1)
-(a0 b1) ctx
-a0 (b1 ctx)
-(b1 ctx) a0
-      ***)
-     rewrite <- ModL.add_assoc' in PR.
-     eapply ModL.add_comm in PR.
-     rewrite <- ModL.add_assoc' in PR.
-     eapply ModL.add_comm in PR.
-     (***
-(b1 ctx) a1
-a1 (b1 ctx)
-(a1 b1) ctx
-ctx (a1 b1)
-      ***)
-     specialize (SIM0 (s1 ++ ctx)). spc SIM0. rewrite Mod.add_list_app in SIM0. eapply SIM0 in PR.
-     eapply ModL.add_comm in PR.
-     rewrite ModL.add_assoc' in PR.
-     eapply ModL.add_comm in PR.
-     rewrite ! Mod.add_list_app in *.
-     assumption.
-   Qed.
-
-
-   Corollary refines2_pairwise
-             (mds0_src mds0_tgt: list Mod.t)
-             (FORALL: List.Forall2 (fun md_src md_tgt => refines2 [md_src] [md_tgt]) mds0_src mds0_tgt)
-     :
-       refines2 mds0_src mds0_tgt.
-   Proof.
-     induction FORALL; ss.
-     hexploit refines2_add.
-     { eapply H0. }
-     { eapply IHFORALL. }
-     i. ss.
-   Qed.
-
-   Lemma refines2_eq (mds0 mds1: list Mod.t)
-     :
-       refines2 mds0 mds1 <-> refines (Mod.add_list mds0) (Mod.add_list mds1).
-   Proof.
-     split.
-     { ii. eapply H0. auto. }
-     { ii. eapply H0. auto. }
-   Qed.
-
-   Lemma refines2_app mhd0 mhd1 mtl0 mtl1
-         (HD: refines2 mhd0 mhd1)
-         (TL: refines2 mtl0 mtl1)
-     :
-       refines2 (mhd0++mtl0) (mhd1++mtl1).
-   Proof.
-     eapply refines2_eq. rewrite ! Mod.add_list_app. etrans.
-     { eapply refines_proper_l. eapply refines2_eq. et. }
-     { eapply refines_proper_r. eapply refines2_eq. et. }
-   Qed.
-
-   Lemma refines2_cons mhd0 mhd1 mtl0 mtl1
-         (HD: refines2 [mhd0] [mhd1])
-         (TL: refines2 mtl0 mtl1)
-     :
-       refines2 (mhd0::mtl0) (mhd1::mtl1).
-   Proof.
-     eapply (refines2_app HD TL).
-   Qed.
-
-   End CONF.
-
-
-
-   (*** horizontal composition ***)
-   Theorem refines_strong_add
-         (md0_src md0_tgt md1_src md1_tgt: Mod.t)
-         (SIM0: refines_strong md0_tgt md0_src)
-         (SIM1: refines_strong md1_tgt md1_src)
-     :
-       <<SIM: refines_strong (ModL.add md0_tgt md1_tgt) (ModL.add md0_src md1_src)>>
-   .
-   Proof.
-     intros CONF. eapply (@refines_add CONF); et.
-   Qed.
-
-   Theorem refines_strong_proper_r
-         (mds0_src mds0_tgt: list Mod.t) (ctx: list Mod.t)
-         (SIM0: refines_strong (Mod.add_list mds0_tgt) (Mod.add_list mds0_src))
-     :
-       <<SIM: refines_strong (ModL.add (Mod.add_list mds0_tgt) (Mod.add_list ctx)) (ModL.add (Mod.add_list mds0_src) (Mod.add_list ctx))>>
-   .
-   Proof.
-     intros CONF. eapply (@refines_proper_r CONF); et.
-   Qed.
-
-   Theorem refines_strong_proper_l
-         (mds0_src mds0_tgt: list Mod.t) (ctx: list Mod.t)
-         (SIM0: refines_strong (Mod.add_list mds0_tgt) (Mod.add_list mds0_src))
-     :
-       <<SIM: refines_strong (ModL.add (Mod.add_list ctx) (Mod.add_list mds0_tgt)) (ModL.add (Mod.add_list ctx) (Mod.add_list mds0_src))>>
-   .
-   Proof.
-     intros CONF. eapply (@refines_proper_l CONF); et.
-   Qed.
-
-   Lemma refines_strong_refines {CONF: EMSConfig}: refines_strong <2= refines.
-   Proof. ii. eapply PR; et. Qed.
-End REFINE.
 
 
 Global Existing Instance Sk.gdefs.
