ems/ModSemE.v
@@ -3,12 +3,11 @@ Require Export sflib.
 Require Export ITreelib.
 Require Export AList.
 Require Import Any.
+Require Import Skeleton.
 
 Set Implicit Arguments.
 
 
-Notation gname := string (only parsing). (*** convention: not capitalized ***)
-Notation mname := string (only parsing). (*** convention: capitalized ***)
 
 Section EVENTSCOMMON.
 
@@ -112,7 +111,7 @@ Module EventsL.
 Section EVENTSL.
 
   Inductive callE: Type -> Type :=
-  | Call (mn: option mname) (fn: gname) (args: Any.t): callE Any.t
+  | Call (mn: mname) (fn: gname) (args: Any.t): callE Any.t
   .
 
   Inductive pE: Type -> Type :=
@@ -147,13 +146,16 @@ Section EVENTSL.
   (*************************** Interpretation *************************)
   (********************************************************************)
 
-  Definition handle_pE {E}: pE ~> stateT p_state (itree E) :=
+  Definition handle_pE `{eventE -< E}: pE ~> stateT p_state (itree E) :=
     fun _ e mps =>
       match e with
       | PPut mn p => Ret (update mps mn p, tt)
-      | PGet mn => Ret (mps, mps mn)
+      | PGet mn => match mn with
+                   | mn_core => triggerUB
+                   | _  => Ret (mps, mps mn)
+                   end
       end.
-  Definition interp_pE {E}: itree (pE +' E) ~> stateT p_state (itree E) :=
+  Definition interp_pE `{eventE -< E}: itree (pE +' E) ~> stateT p_state (itree E) :=
     (* State.interp_state (case_ ((fun _ e s0 => resum_itr (handle_pE e s0)): _ ~> stateT _ _) State.pure_state). *)
     State.interp_state (case_ handle_pE pure_state).
 
